Makefile
@@ -1,0 +1,19 @@
+SRCS    := $(wildcard *.v)
+OBJS := $(SRCS:.v=*.vos)
+
+$(OBJS): Stlc.v Gadgets.v
+	for f in $^; do coqc -vos $$f; done
+
+Stlc.v: Stlc.ott
+	ott -i $< -o $@
+	patch -u $@ -i stlc.patch
+
+.PHONY: ott
+ott: Stlc.v
+
+.PHONY: all
+all: Stlc.v $(OBJS)
+
+.PHONY: clean
+clean:
+	-rm Stlc.v *.vos *.glob *.vo *.vok
